

1. Consider the boundary value problem (12.1)-(12.2) with $f(x) = 1/x$. Using (12.3) prove that $u(x) = -x \log(x)$. This shows that $u \in C^2(0,1)$ but $u(0)$ is not defined and u' , u'' do not exist at $x = 0$ (\Rightarrow : if $f \in C^0(0,1)$, but not $f \in C^0([0,1])$, then u does not belong to $C^0([0,1])$).

For $x \in (0,1)$:

$$u(x) = \int_0^x s(1-x) \frac{1}{s} ds + \int_x^1 x(1-s) \frac{1}{s} ds$$

$$= \int_0^x (1-x) ds + x \int_x^1 \left(\frac{1}{s} - 1\right) ds$$

$$= x(1-x) + x \left(\ln|s| - s \right) \Big|_{s=x}^{s=1}$$

$$= x - x^2 + x(-1 - \ln x + x) = -x \ln x$$

$$u(x) = -x \ln x \in C^2(0,1) : u'(x) = -\ln x - 1, u''(x) = -\frac{1}{x}$$

$$\text{As } x \rightarrow 0^+ : u'(x) \rightarrow \infty, u''(x) \rightarrow -\infty.$$

So u, u' and u'' do not exist at $x = 0$.

4. Cerify the summation by parts formula

$$\sum_{j=0}^{n-1} (w_{j+1} - w_j) v_j = w_n v_n - w_0 v_0 - \sum_{j=0}^{n-1} (v_{j+1} - v_j) w_{j+1},$$

and show that, for $v_h \in V_h^0$,

$$(L_h v_h, v_h)_h = h^{-1} \sum_{j=0}^{n-1} (v_{j+1} - v_j)^2.$$

①.

$$\begin{aligned} \sum_{j=0}^{n-1} (w_{j+1} - w_j) v_j &= \sum_{j=0}^{n-1} w_{j+1} v_j - \sum_{j=0}^{n-1} w_j v_j \\ &= \sum_{j=1}^n w_j v_{j-1} - \sum_{j=0}^{n-1} w_j v_j \\ &= \sum_{j=1}^{n-1} w_j (v_{j-1} - v_j) + w_n v_{n-1} - w_0 v_0 \\ &= - \sum_{j=1}^{n-1} w_j (v_j - v_{j-1}) + w_n v_{n-1} - w_0 v_0 \\ &= - \sum_{j=0}^{n-1} w_{j+1} (v_{j+1} - v_j) + w_n (v_n - v_{n-1}) + w_n v_{n-1} - w_0 v_0 \\ &= w_n v_n - w_0 v_0 - \sum_{j=0}^{n-1} (v_{j+1} - v_j) w_{j+1} \quad \# \end{aligned}$$

②. L_h is defined by $(L_h v_h)_j = - \frac{v_{j+1} - 2v_j + v_{j-1}}{h^2}$, $j=1, \dots, n-1$
and $(u_h, v_h)_h = h \sum_{j=1}^{n-1} u_j v_j$

$$\text{So } (L_h v_h, v_h)_h = h \sum_{j=1}^{n-1} \frac{-v_{j+1} + 2v_j - v_{j-1}}{h^2} v_j = -\frac{1}{h} \sum_{j=1}^{n-1} (v_{j+1} - 2v_j + v_{j-1}) v_j$$

$$- \sum_{j=1}^{n-1} (v_{j+1} - 2v_j + v_{j-1}) v_j = - \sum_{j=1}^{n-1} (v_{j+1} - v_j) v_j + \sum_{j=1}^{n-1} (v_j - v_{j-1}) v_j$$

$$= - \sum_{j=1}^{n-1} (v_{j+1} - v_j) v_j + \sum_{j=0}^{n-2} (v_{j+1} - v_j) v_{j+1}$$

$$= \sum_{j=0}^{n-1} (v_{j+1} - v_j)^2 + (v_1 - v_0) \underset{0}{v_0} - (v_n - v_{n-1}) \underset{0}{v_n}$$

$$\text{Thus, } (L_h v_h, v_h)_h = \frac{1}{h} \sum_{j=0}^{n-1} (v_{j+1} - v_j)^2 \quad \#$$

6. Prove that $G^k(x_j) = hG(x_j, x_k)$, where G is Green's function introduced in (12.4) and G^k is its corresponding discrete counterpart solution of (12.4).

Recall: $G^k \in V_h^0$ as the solution to $L_h G^k = e^k$, where $e^k(x_j) = \begin{cases} 1, & \text{if } k=j \\ 0, & \text{if } k \neq j \end{cases}$

$$G(x, s) = \begin{cases} s(1-x), & 0 \leq s \leq x \\ x(1-s), & x \leq s \leq 1 \end{cases}; \quad L_h(v)(x_j) = -\frac{v(x_{j+1}) - 2v(x_j) + v(x_{j-1}))}{h^2}$$

<pf>

To show $L_h(hG(x_j, x_k)) = \delta_{jk}$ and satisfies boundary condition

① Boundary: $hG(x_0, x_k) = 0$ & $hG(x_n, x_k) = 0$

② $\boxed{j \neq k}$: Fix x_k , $G(x, x_k) = \begin{cases} x_k(1-x), & 0 \leq x_k \leq x \\ x(1-x_k), & x \leq x_k \leq 1 \end{cases}$

Since Green function is a straight line for $j \neq k$

$$L_h(hG(x_j, x_k)) = -\frac{G(x_{j+1}, x_k) - 2G(x_j, x_k) + G(x_{j-1}, x_k))}{h} = 0$$

$$\cdot f(x) = ax + b, \quad x_{j+1} = (j+1)h = jh + h = x_j + h; \quad x_{j-1} = x_j - h$$

$$\cdot f(x_{j+1}) - 2f(x_j) + f(x_{j-1}) = [a(x_j + h) + b] - 2(ax_j + b) + [a(x_j - h) + b] = 0$$

$$\boxed{j=k}: L_h(hG(x_k, x_k)) = -\frac{G(x_{k+1}, x_k) - 2G(x_k, x_k) + G(x_{k-1}, x_k))}{h} \\ = -\frac{-h}{h} = 1$$

$$\dot{f} = x_k(1-x_{k+1}) - 2x_k(1-x_k) + x_{k-1}(1-x_k)$$

$$= x_k(1-x_k-h) - 2x_k + 2x_k^2 + (x_k-h)(1-x_k)$$

$$= x_k - x_k^2 - x_k h - 2x_k + 2x_k^2 + x_k - x_k^2 - h + x_k h = -h$$